src/Hoare.v
@@ -33,9 +33,11 @@ Notation "{< e1 .. e2 , 'PRE' pre 'POST' : r post 'CRASH' crash >} p1" :=
   (forall rx, corr2
    (fun done_ crash_ =>
     (exis (fun e1 => .. (exis (fun e2 =>
-     pre * [[ forall r_,
-             {{ fun done'_ crash'_ => (fun r => post) r_ * [[ done'_ = done_ ]] * [[ crash'_ = crash_ ]]
-             }} rx r_ ]] * [[ (crash)%pred ==> crash_ ]]
+     exists F,
+     F * pre *
+     [[ forall r_,
+        {{ fun done'_ crash'_ => (fun r => F * post) r_ * [[ done'_ = done_ ]] * [[ crash'_ = crash_ ]]
+        }} rx r_ ]] * [[ (F * crash)%pred ==> crash_ ]]
      )) .. ))
    )%pred
    (p1 rx)%pred)
@@ -45,14 +47,15 @@ Notation "{< e1 .. e2 , 'PRE' pre 'POST' : rp post 'CRASH' : rc crash 'IDEM' ide
   (forall rxOK rxREC, corr3
    (fun done_ crashdone_ =>
     (exis (fun e1 => .. (exis (fun e2 =>
-     pre *
+     exists F,
+     F * pre *
      [[ forall r_,
-        {{ fun done'_ crash'_ => (fun rp => post) r_ *
-                                 [[ done'_ = done_ ]] * [[ crash'_ ==> idemcrash ]]
+        {{ fun done'_ crash'_ => (fun rp => F * post) r_ *
+                                 [[ done'_ = done_ ]] * [[ crash'_ ==> F * idemcrash ]]
         }} rxOK r_ ]] *
      [[ forall r_,
-        {{ fun done'_ crash'_ => (fun rc => crash) r_ *
-                                 [[ done'_ = crashdone_ ]] * [[ crash'_ ==> idemcrash ]]
+        {{ fun done'_ crash'_ => (fun rc => F * crash) r_ *
+                                 [[ done'_ = crashdone_ ]] * [[ crash'_ ==> F * idemcrash ]]
         }} rxREC r_ ]]
      )) .. ))
    )%pred
